Result.thy
@@ -2,6 +2,10 @@ theory Result
   imports "HOL-Library.Monad_Syntax"
 begin
 
+section "Definitions"
+
+
+subsection "Types"
 
 datatype error = unknown_register | uninitialized_register | register_override
   | unallocated_address | uninitialized_address
@@ -9,6 +13,8 @@ datatype error = unknown_register | uninitialized_register | register_override
 
 datatype 'a result = ok 'a | err error
 
+
+subsection "Operations"
 
 definition bind :: "'a result \<Rightarrow> ('a \<Rightarrow> 'b result) \<Rightarrow> 'b result" where
   "bind R f = (case R of err e \<Rightarrow> err e | ok x \<Rightarrow> f x)"
@@ -18,7 +24,33 @@ definition return :: "'a \<Rightarrow> 'a result" where
 
 adhoc_overloading
   Monad_Syntax.bind==bind
-(* TODO Monad laws *)
 
+
+fun assert where "assert e True = ok ()" | "assert e False = err e"
+
+
+
+section "Lemmas"
+
+declare bind_def[simp]
+declare return_def[simp]
+
+lemma result_monad_left_identity[simp]: "do {x'\<leftarrow>return x; f x'} = f x"
+  by auto
+
+lemma result_monad_right_identity[simp]: "do {x \<leftarrow> m; return x} = m"
+  by (cases m; simp)
+
+lemma result_monad_associative[simp]: "do {y \<leftarrow> do {x \<leftarrow> (m::'a result); f x}; g y} = do {x \<leftarrow> m; do {y \<leftarrow> f x; g y}}"
+  by (cases m; simp)
+
+lemma result_monad_associative'[simp]: "do {x \<leftarrow> (m::'a result); do {y \<leftarrow> f x; g y}} = do {x \<leftarrow> m; y \<leftarrow> f x; g y}"
+  by simp
+
+lemma assert_inv_simps[simp]: 
+  "assert e P = ok x \<longleftrightarrow> P" 
+  "assert e P = err e' \<longleftrightarrow> \<not>P \<and> e'=e"
+  apply (cases P; simp)
+  by (cases P; auto)
 
 end
