LLVMExamples.thy
@@ -1,0 +1,86 @@
+theory LLVMExamples
+  imports LLVM
+begin
+
+section "Simple Branching"
+
+definition sbmain :: "llvm_instruction_block" where
+  "sbmain = ([
+    alloca ''%1'' i32 (Some 4),
+    alloca ''%2'' i32 (Some 4),
+    alloca ''%3'' i32 (Some 4),
+    alloca ''%4'' i32 (Some 4),
+    alloca ''%5'' i32 (Some 4),
+    store i32 (val (vi32 0)) (ptr (reg ''%1'')) (Some 4),
+    store i32 (val (vi32 1)) (ptr (reg ''%2'')) (Some 4),
+    store i32 (val (vi32 2)) (ptr (reg ''%3'')) (Some 4),
+    load ''%6'' i32 (ptr (reg ''%2'')) (Some 4),
+    add ''%7'' add_nsw i32 (reg ''%6'') (val (vi32 1)),
+    load ''%8'' i32 (ptr (reg ''%3'')) (Some 4),
+    icmp ''%9'' False comp_eq i32 (reg ''%7'') (reg ''%8'')],
+    br_i1 (reg ''%9'') ''10'' ''12''
+  )"
+
+definition sb10 :: "llvm_instruction_block" where
+  "sb10 = ([
+    store i32 (val (vi32 3)) (ptr (reg ''%4'')) (Some 4),
+    load ''%11'' i32 (ptr (reg ''%4'')) (Some 4),
+    store i32 (reg ''%11'') (ptr (reg ''%3'')) (Some 4)],
+    br_label ''14''
+  )"
+
+definition sb12 :: "llvm_instruction_block" where
+  "sb12 = ([
+    store i32 (val (vi32 4)) (ptr (reg ''%5'')) (Some 4),
+    load ''%13'' i32 (ptr (reg ''%5'')) (Some 4),
+    store i32 (reg ''%13'') (ptr (reg ''%3'')) (Some 4)],
+    br_label ''14''
+  )"
+
+definition sb14 :: "llvm_instruction_block" where
+  "sb14 = ([
+    load ''%15'' i32 (ptr (reg ''%3'')) (Some 4)],
+    ret i32 (reg ''%15'')
+  )"
+
+definition simple_branching_main :: "llvm_function" where
+  "simple_branching_main = func (func_def ''main'' i32) sbmain (Mapping.of_alist [(''10'', sb10), (''12'', sb12), (''14'', sb14)])"
+
+(*
+int main() {
+    int y = 1;
+    int x = y?1:0;
+    return x;
+}
+*)
+(*
+define dso_local i32 @main() #0 {
+  %1 = alloca i32, align 4
+  %2 = alloca i32, align 4
+  %3 = alloca i32, align 4
+  %4 = alloca i32, align 4
+  store i32 0, ptr %1, align 4
+  store i32 1, ptr %2, align 4
+  %5 = load i32, ptr %2, align 4
+  %6 = icmp ne i32 %5, 0
+  br i1 %6, label %7, label %9
+
+7:
+  store i32 1, ptr %4, align 4
+  %8 = load i32, ptr %4, align 4
+  br label %10
+
+9:
+  br label %10
+
+10:
+  %11 = phi i32 [ %8, %9 ], [ 0, %9 ]
+  store i32 %11, ptr %3, align 4
+  %12 = load i32, ptr %3, align 4
+  ret i32 %12
+}
+*)
+
+value "execute_function (empty_register_model, empty_memory_model, empty_memory_model) simple_branching_main"
+
+end
